A12Kernel.lean
@@ -232,6 +232,7 @@ import A12Kernel.Elaboration.EnumerationComputationResult
 import A12Kernel.Elaboration.AddressedEnumerationComputation
 import A12Kernel.Elaboration.AddressedEnumerationCascade
 import A12Kernel.Elaboration.AddressedEnumerationFirstFilledComputation
+import A12Kernel.Elaboration.AddressedNumberEnumerationHavingCascade
 import A12Kernel.Elaboration.EnumerationFirstFilledComputation
 import A12Kernel.Elaboration.NumericValidation
 import A12Kernel.Elaboration.ValidationCondition
